src/Definitions.thy
@@ -6,6 +6,10 @@ primrec repeat :: "'a \<Rightarrow> nat \<Rightarrow> 'a list" where
   "repeat a 0 = []"
 | "repeat a (Suc n) = a # repeat a n"
 
+fun update :: "nat \<Rightarrow> 'a \<Rightarrow> 'a list \<Rightarrow> 'a list" where
+  "update 0 x (y # ys) = x # ys"
+| "update (Suc n) x (y # ys) = y # update n x ys"
+| "update _ _ _ = undefined"
 
 datatype election_term = election_term (election_term_of: nat)
 
@@ -18,6 +22,9 @@ definition
 instance ..
 
 end
+
+fun increment_election_term where
+  "increment_election_term t = election_term (election_term_of t + 1)"
 
 datatype node = node (node_of: nat)
 
